Prefix: : <http://www.semanticweb.org/abc/ontologies/2025/2/untitled-ontology-45/>
Prefix: dc: <http://purl.org/dc/elements/1.1/>
Prefix: owl: <http://www.w3.org/2002/07/owl#>
Prefix: rdf: <http://www.w3.org/1999/02/22-rdf-syntax-ns#>
Prefix: rdfs: <http://www.w3.org/2000/01/rdf-schema#>
Prefix: xml: <http://www.w3.org/XML/1998/namespace>
Prefix: xsd: <http://www.w3.org/2001/XMLSchema#>



Ontology: <http://www.semanticweb.org/abc/ontologies/2025/2/untitled-ontology-45/>

Import: <http://purl.obolibrary.org/obo/bfo/2.0/bfo.owl>
Import: <http://www.semanticweb.org/abc/ontologies/2025/2/untitled-ontology-46/>
Import: <http://www.semanticweb.org/abc/ontologies/2025/2/untitled-ontology-47/>

Annotations: 
    rdfs:comment "The Modelling Uncertainties Ontology (MUNO) is a BFO-based mid-level ontology for the annotation and description of modelling uncertainties in many domains. MUNO was built based on the uncertainty matrix by Walker et.al. (2003) and Kwakkel et.al. (2010)."

AnnotationProperty: <http://purl.obolibrary.org/obo/IAO_0000115>

    
AnnotationProperty: <http://purl.obolibrary.org/obo/IAO_0000118>

    
AnnotationProperty: <http://purl.obolibrary.org/obo/IAO_0000600>

    
AnnotationProperty: rdfs:comment

    
AnnotationProperty: rdfs:label

    
Datatype: rdf:PlainLiteral

    
Datatype: xsd:float

    
Datatype: xsd:string

    
ObjectProperty: <http://openenergy-platform.org/ontology/oeo/MUNO_01043>

    Annotations: 
        rdfs:label "models"@de
    
    SubPropertyOf: 
        owl:topObjectProperty
    
    Domain: 
        <http://openenergy-platform.org/ontology/oeo/MUNO_01001>
    
    Range: 
        <http://purl.obolibrary.org/obo/RO_0002577>
    
    
ObjectProperty: <http://openenergy-platform.org/ontology/oeo/MUNO_01045>

    Annotations: 
        rdfs:label "has uncertainty location"@de
    
    SubPropertyOf: 
        owl:topObjectProperty
    
    Domain: 
        <http://openenergy-platform.org/ontology/oeo/MUNO_01002>
    
    Range: 
        <http://openenergy-platform.org/ontology/oeo/MUNO_01054>
    
    
ObjectProperty: <http://openenergy-platform.org/ontology/oeo/MUNO_01046>

    Annotations: 
        rdfs:label "has uncertainty level"@de
    
    SubPropertyOf: 
        owl:topObjectProperty
    
    Domain: 
        <http://openenergy-platform.org/ontology/oeo/MUNO_01002>
    
    Range: 
        <http://openenergy-platform.org/ontology/oeo/MUNO_01048>
    
    
ObjectProperty: <http://purl.obolibrary.org/obo/BFO_0000050>

    
ObjectProperty: <http://purl.obolibrary.org/obo/RO_0000057>

    
ObjectProperty: <http://purl.obolibrary.org/obo/RO_0000087>

    
ObjectProperty: <http://purl.obolibrary.org/obo/RO_0002233>

    
ObjectProperty: <http://purl.obolibrary.org/obo/RO_0002234>

    
ObjectProperty: owl:topObjectProperty

    
DataProperty: <http://openenergy-platform.org/ontology/oeo/MUNO_01053>

    Annotations: 
        <http://purl.obolibrary.org/obo/IAO_0000115> "A data property to indicate a probability value in [0,1] to a shallow level of uncertainty.",
        rdfs:label "has shallow uncertainty value"@de
    
    Domain: 
        <http://openenergy-platform.org/ontology/oeo/MUNO_01049>
    
    Range: 
        xsd:float[>= 0.0f , <= 1.0f]
    
    SubPropertyOf: 
        owl:topDataProperty
    
    
DataProperty: owl:topDataProperty

    
Class: <http://openenergy-platform.org/ontology/oeo/MUNO_01001>

    Annotations: 
        rdfs:label "model"@en
    
    EquivalentTo: 
        <http://purl.obolibrary.org/obo/BFO_0000031>
         and (<http://purl.obolibrary.org/obo/RO_0000087> some <http://openenergy-platform.org/ontology/oeo/MUNO_01024>)
    
    SubClassOf: 
        <http://purl.obolibrary.org/obo/BFO_0000031>,
        <http://openenergy-platform.org/ontology/oeo/MUNO_01043> some <http://purl.obolibrary.org/obo/RO_0002577>
    
    
Class: <http://openenergy-platform.org/ontology/oeo/MUNO_01002>

    Annotations: 
        <http://purl.obolibrary.org/obo/IAO_0000115> "Uncertainty is a quality of a model of a system or of the model’s calculation’s output data that expresses any departure from the ideal of representing complete definite knowledge about the system. Definite knowledge of a system implies that one can predict its behaviour accurately under all circumstances for those aspects that are within the scope of the model.",
        rdfs:label "uncertainty"@en
    
    SubClassOf: 
        <http://purl.obolibrary.org/obo/BFO_0000019>
    
    
Class: <http://openenergy-platform.org/ontology/oeo/MUNO_01024>

    Annotations: 
        rdfs:label "model role"@en
    
    SubClassOf: 
        <http://purl.obolibrary.org/obo/BFO_0000023>
    
    
Class: <http://openenergy-platform.org/ontology/oeo/MUNO_01025>

    Annotations: 
        rdfs:label "model component role"@en
    
    SubClassOf: 
        <http://purl.obolibrary.org/obo/BFO_0000023>
    
    
Class: <http://openenergy-platform.org/ontology/oeo/MUNO_01026>

    Annotations: 
        rdfs:label "location of uncertainty role"@en
    
    SubClassOf: 
        <http://purl.obolibrary.org/obo/BFO_0000023>
    
    
Class: <http://openenergy-platform.org/ontology/oeo/MUNO_01029>

    Annotations: 
        rdfs:label "input data"@en
    
    EquivalentTo: 
        <http://purl.obolibrary.org/obo/IAO_0000100>
         and (<http://purl.obolibrary.org/obo/RO_0000087> some <http://openenergy-platform.org/ontology/oeo/MUNO_01057>)
    
    SubClassOf: 
        <http://purl.obolibrary.org/obo/RO_0000087> some <http://openenergy-platform.org/ontology/oeo/MUNO_01026>
    
    
Class: <http://openenergy-platform.org/ontology/oeo/MUNO_01030>

    Annotations: 
        rdfs:label "output data"@en
    
    EquivalentTo: 
        <http://purl.obolibrary.org/obo/IAO_0000100>
         and (<http://purl.obolibrary.org/obo/RO_0000087> some <http://openenergy-platform.org/ontology/oeo/MUNO_01058>)
    
    SubClassOf: 
        <http://purl.obolibrary.org/obo/RO_0000087> some <http://openenergy-platform.org/ontology/oeo/MUNO_01026>
    
    
Class: <http://openenergy-platform.org/ontology/oeo/MUNO_01031>

    Annotations: 
        rdfs:label "endogenous modelling parameter"@en
    
    SubClassOf: 
        <http://purl.obolibrary.org/obo/IAO_0000027>,
        <http://purl.obolibrary.org/obo/RO_0000087> some <http://openenergy-platform.org/ontology/oeo/MUNO_01025>,
        <http://purl.obolibrary.org/obo/RO_0000087> some <http://openenergy-platform.org/ontology/oeo/MUNO_01026>
    
    
Class: <http://openenergy-platform.org/ontology/oeo/MUNO_01032>

    Annotations: 
        rdfs:label "exogenous modelling parameter"@en
    
    SubClassOf: 
        <http://purl.obolibrary.org/obo/IAO_0000027>,
        <http://purl.obolibrary.org/obo/RO_0000087> some <http://openenergy-platform.org/ontology/oeo/MUNO_01025>,
        <http://purl.obolibrary.org/obo/RO_0000087> some <http://openenergy-platform.org/ontology/oeo/MUNO_01026>
    
    
Class: <http://openenergy-platform.org/ontology/oeo/MUNO_01033>

    Annotations: 
        <http://purl.obolibrary.org/obo/IAO_0000115> "A model scope is a generically dependent continuant that represents the demarcation of aspects of the real world system that are included in the model from those that are not included.",
        <http://purl.obolibrary.org/obo/IAO_0000118> "model system boundary"@en,
        <http://purl.obolibrary.org/obo/IAO_0000600> "The model scope is often determined by the problem to be solved by the model and the chosen framing. It is also sometimes referred to as 'context' or seen as part of the 'conceptual model'.",
        rdfs:label "model scope"
    
    SubClassOf: 
        <http://purl.obolibrary.org/obo/BFO_0000031>,
        <http://purl.obolibrary.org/obo/RO_0000087> some <http://openenergy-platform.org/ontology/oeo/MUNO_01025>,
        <http://purl.obolibrary.org/obo/RO_0000087> some <http://openenergy-platform.org/ontology/oeo/MUNO_01026>
    
    
Class: <http://openenergy-platform.org/ontology/oeo/MUNO_01034>

    Annotations: 
        rdfs:label "model implementation"@en
    
    SubClassOf: 
        <http://purl.obolibrary.org/obo/BFO_0000031>,
        <http://purl.obolibrary.org/obo/RO_0000087> some <http://openenergy-platform.org/ontology/oeo/MUNO_01025>
    
    
Class: <http://openenergy-platform.org/ontology/oeo/MUNO_01035>

    Annotations: 
        rdfs:label "model structure"@en
    
    SubClassOf: 
        <http://purl.obolibrary.org/obo/BFO_0000031>,
        <http://purl.obolibrary.org/obo/RO_0000087> some <http://openenergy-platform.org/ontology/oeo/MUNO_01025>,
        <http://purl.obolibrary.org/obo/RO_0000087> some <http://openenergy-platform.org/ontology/oeo/MUNO_01026>
    
    
Class: <http://openenergy-platform.org/ontology/oeo/MUNO_01036>

    Annotations: 
        <http://purl.obolibrary.org/obo/IAO_0000115> "A conceptual model is a generically dependent continuant that specifies variables and relationships inside the system boundaries to represent a system in a simplified way. It has the model role.",
        <http://purl.obolibrary.org/obo/IAO_0000600> "The conceptual model can provide the interpretation of a computer model based on the conceptual model.",
        rdfs:label "conceptual model"@en
    
    SubClassOf: 
        <http://purl.obolibrary.org/obo/BFO_0000031>,
        <http://purl.obolibrary.org/obo/RO_0000087> some <http://openenergy-platform.org/ontology/oeo/MUNO_01024>,
        <http://purl.obolibrary.org/obo/RO_0000087> some <http://openenergy-platform.org/ontology/oeo/MUNO_01025>,
        <http://purl.obolibrary.org/obo/RO_0000087> some <http://openenergy-platform.org/ontology/oeo/MUNO_01026>
    
    
Class: <http://openenergy-platform.org/ontology/oeo/MUNO_01037>

    Annotations: 
        rdfs:label "computer model"@en
    
    SubClassOf: 
        <http://purl.obolibrary.org/obo/BFO_0000031>,
        <http://purl.obolibrary.org/obo/RO_0000087> some <http://openenergy-platform.org/ontology/oeo/MUNO_01024>
    
    
Class: <http://openenergy-platform.org/ontology/oeo/MUNO_01038>

    Annotations: 
        rdfs:label "model component"@en
    
    EquivalentTo: 
        <http://purl.obolibrary.org/obo/BFO_0000031>
         and (<http://purl.obolibrary.org/obo/RO_0000087> some <http://openenergy-platform.org/ontology/oeo/MUNO_01025>)
    
    SubClassOf: 
        <http://purl.obolibrary.org/obo/BFO_0000031>,
        <http://purl.obolibrary.org/obo/BFO_0000050> some <http://openenergy-platform.org/ontology/oeo/MUNO_01001>
    
    
Class: <http://openenergy-platform.org/ontology/oeo/MUNO_01039>

    Annotations: 
        <http://purl.obolibrary.org/obo/IAO_0000115> "Epistemic uncertainty is an uncertainty of a model of a system that exists due to incomplete knowledge or incorrect beliefs about the system.",
        <http://purl.obolibrary.org/obo/IAO_0000118> "epistemological uncertainty",
        rdfs:label "epistemic uncertainty"@de
    
    SubClassOf: 
        <http://openenergy-platform.org/ontology/oeo/MUNO_01002>
    
    
Class: <http://openenergy-platform.org/ontology/oeo/MUNO_01040>

    Annotations: 
        <http://purl.obolibrary.org/obo/IAO_0000115> "Aleatory uncertainty is an uncertainty of a model of a system that exists due to an inherent variability within the system. It is caused by e.g. randomness by nature, human, social or cultural behaviour or technological surprises.",
        <http://purl.obolibrary.org/obo/IAO_0000118> "ontic uncertainty",
        <http://purl.obolibrary.org/obo/IAO_0000118> "ontological uncertainty",
        rdfs:label "aleatory uncertianty"@de
    
    SubClassOf: 
        <http://openenergy-platform.org/ontology/oeo/MUNO_01002>
    
    
Class: <http://openenergy-platform.org/ontology/oeo/MUNO_01041>

    Annotations: 
        <http://purl.obolibrary.org/obo/IAO_0000115> "Ambiguous uncertainty is an uncertainty of a model of a system due to the presence of various frames of reference about a phenomenon related to the system. It is caused by e.g. due to different perceptions, interpretations or values of stakeholders.",
        rdfs:label "ambiguous uncertainty"@de
    
    SubClassOf: 
        <http://openenergy-platform.org/ontology/oeo/MUNO_01002>
    
    
Class: <http://openenergy-platform.org/ontology/oeo/MUNO_01048>

    Annotations: 
        <http://purl.obolibrary.org/obo/IAO_0000115> "Level of model uncertainty is a quality of a model that represents the degree or severity of an uncertainty.",
        rdfs:label "level of uncertainty"@de
    
    SubClassOf: 
        <http://purl.obolibrary.org/obo/BFO_0000019>
    
    
Class: <http://openenergy-platform.org/ontology/oeo/MUNO_01049>

    Annotations: 
        <http://purl.obolibrary.org/obo/IAO_0000115> "Shallow uncertainty is a level of uncertainty that allows to enumerate multiple alternatives and provide probabilities (subjective or objective).",
        rdfs:label "shallow uncertainty"@de
    
    SubClassOf: 
        <http://openenergy-platform.org/ontology/oeo/MUNO_01048>
    
    
Class: <http://openenergy-platform.org/ontology/oeo/MUNO_01050>

    Annotations: 
        <http://purl.obolibrary.org/obo/IAO_0000115> "Medium uncertainty is a level of uncertainty that allows to enumerate multiple alternatives and rank order the alternatives in terms of perceived likelihood, without being able to number the likelihood.",
        rdfs:label "medium uncertainty"@de
    
    SubClassOf: 
        <http://openenergy-platform.org/ontology/oeo/MUNO_01048>
    
    
Class: <http://openenergy-platform.org/ontology/oeo/MUNO_01051>

    Annotations: 
        <http://purl.obolibrary.org/obo/IAO_0000115> "Deep uncertainty is a level of uncertainty that allows to enumerate multiple alternatives without being able to rank order the alternatives in terms of how likely or plausible they are judged to be.",
        rdfs:label "deep uncertainty"@de
    
    SubClassOf: 
        <http://openenergy-platform.org/ontology/oeo/MUNO_01048>
    
    
Class: <http://openenergy-platform.org/ontology/oeo/MUNO_01052>

    Annotations: 
        <http://purl.obolibrary.org/obo/IAO_0000115> "Recognized ignorance is a level of uncertainty that is so severe that one is unable to enumerate multiple alternatives, while admitting the possibility of being surprised.",
        rdfs:label "recognized ignorance"@de
    
    SubClassOf: 
        <http://openenergy-platform.org/ontology/oeo/MUNO_01048>
    
    
Class: <http://openenergy-platform.org/ontology/oeo/MUNO_01054>

    Annotations: 
        <http://purl.obolibrary.org/obo/IAO_0000115> "A model uncertainty location is a generically dependent continuant that has the role to be a location of uncertainty.",
        rdfs:label "location of uncertainty"@de
    
    EquivalentTo: 
        <http://purl.obolibrary.org/obo/BFO_0000031>
         and (<http://purl.obolibrary.org/obo/RO_0000087> some <http://openenergy-platform.org/ontology/oeo/MUNO_01026>)
    
    
Class: <http://openenergy-platform.org/ontology/oeo/MUNO_01057>

    Annotations: 
        rdfs:label "input data role"@de
    
    SubClassOf: 
        <http://purl.obolibrary.org/obo/BFO_0000023>
    
    
Class: <http://openenergy-platform.org/ontology/oeo/MUNO_01058>

    Annotations: 
        rdfs:label "output data role"@de
    
    SubClassOf: 
        <http://purl.obolibrary.org/obo/BFO_0000023>
    
    
Class: <http://openenergy-platform.org/ontology/oeo/MUNO_01059>

    Annotations: 
        rdfs:label "model calculation"@de
    
    SubClassOf: 
        <http://purl.obolibrary.org/obo/BFO_0000015>,
        <http://purl.obolibrary.org/obo/RO_0000057> some <http://openenergy-platform.org/ontology/oeo/MUNO_01037>,
        <http://purl.obolibrary.org/obo/RO_0002233> some <http://openenergy-platform.org/ontology/oeo/MUNO_01029>,
        <http://purl.obolibrary.org/obo/RO_0002234> some <http://openenergy-platform.org/ontology/oeo/MUNO_01030>
    
    
Class: <http://purl.obolibrary.org/obo/BFO_0000002>

    
Class: <http://purl.obolibrary.org/obo/BFO_0000015>

    
Class: <http://purl.obolibrary.org/obo/BFO_0000019>

    
Class: <http://purl.obolibrary.org/obo/BFO_0000023>

    
Class: <http://purl.obolibrary.org/obo/BFO_0000031>

    
Class: <http://purl.obolibrary.org/obo/BFO_0000040>

    
Class: <http://purl.obolibrary.org/obo/IAO_0000027>

    
Class: <http://purl.obolibrary.org/obo/IAO_0000030>

    SubClassOf: 
        <http://purl.obolibrary.org/obo/BFO_0000031>
    
    
Class: <http://purl.obolibrary.org/obo/IAO_0000100>

    
Class: <http://purl.obolibrary.org/obo/RO_0002577>

    
