Prefix: : <https://raw.githubusercontent.com/stap-m/muno/main/src/muno.owl/>
Prefix: dc: <http://purl.org/dc/elements/1.1/>
Prefix: owl: <http://www.w3.org/2002/07/owl#>
Prefix: rdf: <http://www.w3.org/1999/02/22-rdf-syntax-ns#>
Prefix: rdfs: <http://www.w3.org/2000/01/rdf-schema#>
Prefix: xml: <http://www.w3.org/XML/1998/namespace>
Prefix: xsd: <http://www.w3.org/2001/XMLSchema#>



Ontology: <https://raw.githubusercontent.com/stap-m/muno/main/src/muno.owl/>
<https://raw.githubusercontent.com/stap-m/muno/dev/src/muno.owl/>
Import: <http://purl.obolibrary.org/obo/bfo/2020/bfo-core.owl>
Import: <http://www.semanticweb.org/abc/ontologies/2025/2/untitled-ontology-46/>
Import: <http://www.semanticweb.org/abc/ontologies/2025/2/untitled-ontology-47/>

Annotations: 
    dc:contributor "Fabian Neuhaus",
    dc:contributor "Mirjam Stappel",
    dc:contributor "Till Mossakowski",
    <http://purl.org/dc/terms/license> "Creative Commons Attribution 4.0 International (CC-BY-4.0)",
    <http://purl.org/dc/terms/title> "Modelling Uncertainties Ontology",
    rdfs:comment "The Modelling Uncertainties Ontology (MUNO) is a BFO-based mid-level ontology for the annotation and description of modelling uncertainties in many domains. MUNO was built based on the uncertainty matrix by Walker et.al. (2003) and Kwakkel et.al. (2010)."

AnnotationProperty: <http://purl.obolibrary.org/obo/IAO_0000115>

    
AnnotationProperty: <http://purl.obolibrary.org/obo/IAO_0000118>

    
AnnotationProperty: <http://purl.obolibrary.org/obo/IAO_0000600>

    
AnnotationProperty: <http://purl.org/dc/terms/license>

    
AnnotationProperty: <http://purl.org/dc/terms/title>

    
AnnotationProperty: dc:contributor

    
AnnotationProperty: rdfs:comment

    
AnnotationProperty: rdfs:label

    
Datatype: rdf:PlainLiteral

    
Datatype: xsd:float

    
Datatype: xsd:string

    
ObjectProperty: <http://purl.obolibrary.org/obo/BFO_0000050>

    
ObjectProperty: <http://purl.obolibrary.org/obo/RO_0000052>

    
ObjectProperty: <http://purl.obolibrary.org/obo/RO_0000053>

    
ObjectProperty: <http://purl.obolibrary.org/obo/RO_0000057>

    
ObjectProperty: <http://purl.obolibrary.org/obo/RO_0002233>

    
ObjectProperty: <http://purl.obolibrary.org/obo/RO_0002234>

    
ObjectProperty: <http://purl.obolibrary.org/obo/RO_0002352>

    
ObjectProperty: <http://purl.obolibrary.org/obo/RO_0002353>

    
ObjectProperty: MUNO_01043

    Annotations: 
        <http://purl.obolibrary.org/obo/IAO_0000115> "A relation between a model and a system where the model represents the system and its behaviours in a simplified or idealised way.",
        rdfs:label "models"@en
    
    SubPropertyOf: 
        owl:topObjectProperty
    
    Domain: 
        MUNO_01001
    
    Range: 
        <http://purl.obolibrary.org/obo/RO_0002577>
    
    
ObjectProperty: MUNO_01046

    Annotations: 
        rdfs:comment "A relation between a (type of) uncertainty and a level of uncertainty where the level indicates the severity of the uncertainty.",
        rdfs:label "has uncertainty level"@en
    
    SubPropertyOf: 
        owl:topObjectProperty
    
    Domain: 
        MUNO_01002
    
    Range: 
        MUNO_01048
    
    
ObjectProperty: MUNO_01065

    Annotations: 
        <http://purl.obolibrary.org/obo/IAO_0000115> "A relation between a level of uncertainty and a (type of) uncertainty.",
        rdfs:label "uncertainty level of"@de
    
    SubPropertyOf: 
        owl:topObjectProperty
    
    Domain: 
        MUNO_01048
    
    Range: 
        MUNO_01002
    
    
ObjectProperty: owl:topObjectProperty

    
DataProperty: MUNO_01053

    Annotations: 
        <http://purl.obolibrary.org/obo/IAO_0000115> "A data property to indicate the uncertainty value in [0,1] to a shallow epistemic uncertainty. A value of 0 indicate no uncertainty, i.e. 100% probability. A value of 1 indicates full uncertainty, i.e. 0% probability.",
        rdfs:label "has shallow uncertainty value"@en
    
    Domain: 
        MUNO_01049
         and (MUNO_01065 some MUNO_01039)
    
    Range: 
        xsd:float[>= 0.0f , <= 1.0f]
    
    SubPropertyOf: 
        owl:topDataProperty
    
    
DataProperty: owl:topDataProperty

    
Class: <http://purl.obolibrary.org/obo/BFO_0000002>

    
Class: <http://purl.obolibrary.org/obo/BFO_0000015>

    
Class: <http://purl.obolibrary.org/obo/BFO_0000019>

    
Class: <http://purl.obolibrary.org/obo/BFO_0000023>

    
Class: <http://purl.obolibrary.org/obo/BFO_0000031>

    
Class: <http://purl.obolibrary.org/obo/BFO_0000040>

    
Class: <http://purl.obolibrary.org/obo/IAO_0000027>

    
Class: <http://purl.obolibrary.org/obo/IAO_0000030>

    SubClassOf: 
        <http://purl.obolibrary.org/obo/BFO_0000031>
    
    
Class: <http://purl.obolibrary.org/obo/IAO_0000100>

    
Class: <http://purl.obolibrary.org/obo/RO_0002577>

    
Class: MUNO_01001

    Annotations: 
        <http://purl.obolibrary.org/obo/IAO_0000115> "A model is a generically  dependent continuant for representing (knowledge about) a system and its behaviours in a simplified or idealised way. It has the model role.",
        rdfs:label "model"@en
    
    EquivalentTo: 
        <http://purl.obolibrary.org/obo/BFO_0000031>
         and (<http://purl.obolibrary.org/obo/RO_0000053> some MUNO_01024)
    
    SubClassOf: 
        <http://purl.obolibrary.org/obo/BFO_0000031>,
        MUNO_01043 some <http://purl.obolibrary.org/obo/RO_0002577>
    
    
Class: MUNO_01002

    Annotations: 
        <http://purl.obolibrary.org/obo/IAO_0000115> "Uncertainty is a quality of a model of a system or of the model’s calculation’s output data that expresses any departure from the ideal of representing complete definite knowledge about the system. Definite knowledge of a system implies that one can predict its behaviour accurately under all circumstances for those aspects that are within the scope of the model.",
        rdfs:label "uncertainty"@en
    
    SubClassOf: 
        <http://purl.obolibrary.org/obo/BFO_0000019>,
        <http://purl.obolibrary.org/obo/RO_0000052> some MUNO_01001,
        <http://purl.obolibrary.org/obo/RO_0000052> some MUNO_01054
    
    
Class: MUNO_01024

    Annotations: 
        <http://purl.obolibrary.org/obo/IAO_0000115> "A model role is a role of a generically  dependent continuant for representing (knowledge about) a system and its behaviours in a simplified or idealised way.",
        rdfs:label "model role"@en
    
    SubClassOf: 
        <http://purl.obolibrary.org/obo/BFO_0000023>,
        <http://purl.obolibrary.org/obo/RO_0000052> some MUNO_01001
    
    
Class: MUNO_01025

    Annotations: 
        <http://purl.obolibrary.org/obo/IAO_0000115> "A model component role is the role of a generically dependent continuant that is part of a model.",
        rdfs:label "model component role"@en
    
    SubClassOf: 
        <http://purl.obolibrary.org/obo/BFO_0000023>,
        <http://purl.obolibrary.org/obo/RO_0000052> some MUNO_01038
    
    
Class: MUNO_01026

    Annotations: 
        <http://purl.obolibrary.org/obo/IAO_0000115> "Location of uncertainty role is a role of an entity in which a model uncertainty is located in.",
        rdfs:label "location of uncertainty role"@en
    
    SubClassOf: 
        <http://purl.obolibrary.org/obo/BFO_0000023>,
        <http://purl.obolibrary.org/obo/RO_0000052> some MUNO_01054
    
    
Class: MUNO_01029

    Annotations: 
        <http://purl.obolibrary.org/obo/IAO_0000115> "Input data is a data set that is used as input data in a model calculation. It has the input data role.",
        rdfs:label "input data"@en
    
    EquivalentTo: 
        <http://purl.obolibrary.org/obo/IAO_0000100>
         and (<http://purl.obolibrary.org/obo/RO_0000053> some MUNO_01057)
    
    SubClassOf: 
        <http://purl.obolibrary.org/obo/RO_0000053> some MUNO_01026,
        <http://purl.obolibrary.org/obo/RO_0002352> some MUNO_01059
    
    
Class: MUNO_01030

    Annotations: 
        <http://purl.obolibrary.org/obo/IAO_0000115> "Output data is a data set that is the output result of a model calculation. It has the output data role.",
        rdfs:label "output data"@en
    
    EquivalentTo: 
        <http://purl.obolibrary.org/obo/IAO_0000100>
         and (<http://purl.obolibrary.org/obo/RO_0000053> some MUNO_01058)
    
    SubClassOf: 
        <http://purl.obolibrary.org/obo/RO_0000053> some MUNO_01026,
        <http://purl.obolibrary.org/obo/RO_0002353> some MUNO_01059
    
    
Class: MUNO_01031

    Annotations: 
        <http://purl.obolibrary.org/obo/IAO_0000115> "An endogenous modelling parameter is a data item that is a fixed parameter inside a computer model.",
        rdfs:label "endogenous modelling parameter"@en
    
    SubClassOf: 
        <http://purl.obolibrary.org/obo/IAO_0000027>,
        <http://purl.obolibrary.org/obo/RO_0000053> some MUNO_01025,
        <http://purl.obolibrary.org/obo/RO_0000053> some MUNO_01026
    
    
Class: MUNO_01032

    Annotations: 
        <http://purl.obolibrary.org/obo/IAO_0000115> "An exogenous modelling parameter is a data item that is used as input to the model but is defined outside the model (exogenous) and can be changed to reflect different external developments.",
        rdfs:label "exogenous modelling parameter"@en
    
    SubClassOf: 
        <http://purl.obolibrary.org/obo/IAO_0000027>,
        <http://purl.obolibrary.org/obo/RO_0000053> some MUNO_01025,
        <http://purl.obolibrary.org/obo/RO_0000053> some MUNO_01026
    
    
Class: MUNO_01033

    Annotations: 
        <http://purl.obolibrary.org/obo/IAO_0000115> "A model scope is a generically dependent continuant that represents the demarcation of aspects of the real world system that are included in the model from those that are not included.",
        <http://purl.obolibrary.org/obo/IAO_0000118> "model system boundary"@en,
        <http://purl.obolibrary.org/obo/IAO_0000600> "The model scope is often determined by the problem to be solved by the model and the chosen framing. It is also sometimes referred to as 'system boundary' or 'context' or seen as part of the 'conceptual model'.",
        rdfs:label "model scope"
    
    SubClassOf: 
        <http://purl.obolibrary.org/obo/BFO_0000031>,
        <http://purl.obolibrary.org/obo/RO_0000053> some MUNO_01025,
        <http://purl.obolibrary.org/obo/RO_0000053> some MUNO_01026
    
    
Class: MUNO_01034

    Annotations: 
        <http://purl.obolibrary.org/obo/IAO_0000115> "A technical model implementation is a generically dependent continuant that is the part of a computer model that refers to the applied hardware and software.",
        rdfs:label "technical model implementation"@en
    
    SubClassOf: 
        <http://purl.obolibrary.org/obo/BFO_0000031>,
        <http://purl.obolibrary.org/obo/RO_0000053> some MUNO_01025
    
    
Class: MUNO_01035

    Annotations: 
        <http://purl.obolibrary.org/obo/IAO_0000115> "The model structure is a generically dependent continuant that is part of a computer model and represents generic design choices of the algorithms.",
        rdfs:label "model structure"@en
    
    SubClassOf: 
        <http://purl.obolibrary.org/obo/BFO_0000031>,
        <http://purl.obolibrary.org/obo/RO_0000053> some MUNO_01025,
        <http://purl.obolibrary.org/obo/RO_0000053> some MUNO_01026
    
    
Class: MUNO_01036

    Annotations: 
        <http://purl.obolibrary.org/obo/IAO_0000115> "A conceptual model is a generically dependent continuant that specifies variables and relationships inside the system boundaries to represent a system in a simplified way. It has the model role.",
        <http://purl.obolibrary.org/obo/IAO_0000600> "The conceptual model can provide the interpretation of a computer model based on the conceptual model.",
        rdfs:label "conceptual model"@en
    
    SubClassOf: 
        <http://purl.obolibrary.org/obo/BFO_0000031>,
        <http://purl.obolibrary.org/obo/RO_0000053> some MUNO_01024,
        <http://purl.obolibrary.org/obo/RO_0000053> some MUNO_01025,
        <http://purl.obolibrary.org/obo/RO_0000053> some MUNO_01026
    
    
Class: MUNO_01037

    Annotations: 
        <http://purl.obolibrary.org/obo/IAO_0000115> "A computer model is a generically dependent continuant that is the implementation of a conceptual model in computer code. It has the model role.",
        rdfs:label "computer model"@en
    
    SubClassOf: 
        <http://purl.obolibrary.org/obo/BFO_0000031>,
        <http://purl.obolibrary.org/obo/RO_0000053> some MUNO_01024
    
    
Class: MUNO_01038

    Annotations: 
        <http://purl.obolibrary.org/obo/IAO_0000115> "A model component is a generically dependent continuant that is part of a computer model. It has the model component role.",
        rdfs:label "model component"@en
    
    EquivalentTo: 
        <http://purl.obolibrary.org/obo/BFO_0000031>
         and (<http://purl.obolibrary.org/obo/RO_0000053> some MUNO_01025)
    
    SubClassOf: 
        <http://purl.obolibrary.org/obo/BFO_0000031>,
        <http://purl.obolibrary.org/obo/BFO_0000050> some MUNO_01001
    
    
Class: MUNO_01039

    Annotations: 
        <http://purl.obolibrary.org/obo/IAO_0000115> "Epistemic uncertainty is an uncertainty of a model of a system that exists due to incomplete knowledge or incorrect beliefs about the system.",
        <http://purl.obolibrary.org/obo/IAO_0000118> "epistemological uncertainty",
        rdfs:label "epistemic uncertainty"@en
    
    SubClassOf: 
        MUNO_01002
    
    
Class: MUNO_01040

    Annotations: 
        <http://purl.obolibrary.org/obo/IAO_0000115> "Aleatory uncertainty is an uncertainty of a model of a system that exists due to an inherent variability within the system. It is caused by e.g. randomness by nature, human, social or cultural behaviour or technological surprises.",
        <http://purl.obolibrary.org/obo/IAO_0000118> "ontic uncertainty",
        <http://purl.obolibrary.org/obo/IAO_0000118> "ontological uncertainty",
        rdfs:label "aleatory uncertianty"@en
    
    SubClassOf: 
        MUNO_01002
    
    
Class: MUNO_01041

    Annotations: 
        <http://purl.obolibrary.org/obo/IAO_0000115> "Ambiguous uncertainty is an uncertainty of a model of a system due to the presence of various frames of reference about a phenomenon related to the system. It is caused by e.g. due to different perceptions, interpretations or values of stakeholders.",
        rdfs:label "ambiguous uncertainty"@en
    
    SubClassOf: 
        MUNO_01002
    
    
Class: MUNO_01048

    Annotations: 
        <http://purl.obolibrary.org/obo/IAO_0000115> "Level of model uncertainty is a quality of a model that represents the degree or severity of an uncertainty.",
        rdfs:label "level of uncertainty"@en
    
    SubClassOf: 
        <http://purl.obolibrary.org/obo/BFO_0000019>,
        <http://purl.obolibrary.org/obo/RO_0000052> some MUNO_01001,
        <http://purl.obolibrary.org/obo/RO_0000052> some MUNO_01054
    
    
Class: MUNO_01049

    Annotations: 
        <http://purl.obolibrary.org/obo/IAO_0000115> "Shallow uncertainty is a level of uncertainty that allows to enumerate multiple alternatives and provide probabilities (subjective or objective).",
        rdfs:label "shallow uncertainty"@en
    
    SubClassOf: 
        MUNO_01048
    
    
Class: MUNO_01050

    Annotations: 
        <http://purl.obolibrary.org/obo/IAO_0000115> "Medium uncertainty is a level of uncertainty that allows to enumerate multiple alternatives and rank order the alternatives in terms of perceived likelihood, without being able to number the likelihood.",
        rdfs:label "medium uncertainty"@en
    
    SubClassOf: 
        MUNO_01048
    
    
Class: MUNO_01051

    Annotations: 
        <http://purl.obolibrary.org/obo/IAO_0000115> "Deep uncertainty is a level of uncertainty that allows to enumerate multiple alternatives without being able to rank order the alternatives in terms of how likely or plausible they are judged to be.",
        rdfs:label "deep uncertainty"@en
    
    SubClassOf: 
        MUNO_01048
    
    
Class: MUNO_01052

    Annotations: 
        <http://purl.obolibrary.org/obo/IAO_0000115> "Recognized ignorance is a level of uncertainty that is so severe that one is unable to enumerate multiple alternatives, while admitting the possibility of being surprised.",
        rdfs:label "recognized ignorance"@en
    
    SubClassOf: 
        MUNO_01048
    
    
Class: MUNO_01054

    Annotations: 
        <http://purl.obolibrary.org/obo/IAO_0000115> "A model uncertainty location is a generically dependent continuant that has the role to be a location of uncertainty.",
        rdfs:label "location of uncertainty"@en
    
    EquivalentTo: 
        <http://purl.obolibrary.org/obo/BFO_0000031>
         and (<http://purl.obolibrary.org/obo/RO_0000053> some MUNO_01026)
    
    
Class: MUNO_01057

    Annotations: 
        <http://purl.obolibrary.org/obo/IAO_0000115> "Input data role is the role of a data set that is used as input to a model calculation.",
        rdfs:label "input data role"@en
    
    SubClassOf: 
        <http://purl.obolibrary.org/obo/BFO_0000023>,
        <http://purl.obolibrary.org/obo/RO_0000052> some <http://purl.obolibrary.org/obo/IAO_0000100>
    
    
Class: MUNO_01058

    Annotations: 
        <http://purl.obolibrary.org/obo/IAO_0000115> "Output data role is the role of a data set that is the output result of a model calculation.",
        rdfs:label "output data role"@en
    
    SubClassOf: 
        <http://purl.obolibrary.org/obo/BFO_0000023>,
        <http://purl.obolibrary.org/obo/RO_0000052> some <http://purl.obolibrary.org/obo/IAO_0000030>
    
    
Class: MUNO_01059

    Annotations: 
        <http://purl.obolibrary.org/obo/IAO_0000115> "A model calculation is a process of solving mathematical equations of a model.",
        rdfs:label "model calculation"@en
    
    SubClassOf: 
        <http://purl.obolibrary.org/obo/BFO_0000015>,
        <http://purl.obolibrary.org/obo/RO_0000057> some MUNO_01037,
        <http://purl.obolibrary.org/obo/RO_0002233> some MUNO_01029,
        <http://purl.obolibrary.org/obo/RO_0002234> some MUNO_01030
    
    
